\documentclass[11pt,a4paper]{article}
\usepackage{amsmath,a4wide,listings,color}

\usepackage{hyperref}

\lstdefinelanguage{GAMS}
{
	basicstyle=\ttfamily\tiny,
	sensitive = false,
  morekeywords= {Set, Alias, Parameters},%
   sensitive=f,%
   %morecomment=[s]{*}
   keywordstyle = \bfseries
  }

\begin{document}

\lstset{language=GAMS,
%frame=shadowbox, rulesepcolor=\color{blue}
}


\section{The simple monopoly}

We begin with a static monopoly with one technology. The monopolist has the following objective function:

\begin{equation*}
	\max_q\Pi = (\alpha-\beta q)q - cq 
\end{equation*}

subject to

\begin{eqnarray*}
	q - K &\leq& 0\\
	q &\geq& 0 
\end{eqnarray*}
 
We get the following Lagrangian.

\begin{equation*}
	\mathcal{L}(q,\lambda)= (\alpha-\beta q)q - cq -\lambda(q-K)
\end{equation*}

The KKT Conditions are as follows.

\begin{eqnarray*}
	0 \leq -\alpha + 2\beta q + c + \lambda &\bot& q \geq 0\\
	0 \leq -q + K &\bot& \lambda \geq 0
\end{eqnarray*}

Consider the numeric example where $\alpha=100$, $\beta=0.75$ and $c=3$. We compare the results with a quantity restricition of $K=55$, and then without it.

\subsection*{ex$\_$monopoly.gms}

\lstinputlisting{ex_monopoly.gms}

\subsection*{ex$\_$monopoly.lst}

\lstinputlisting{ex_monopoly.lst}

\section{The simple monopoly goes dynamic}


We consider again the monopolist who produces with one technology. Now, we extend the time horizon to two stages, and allow for an investment in $t=0$, which translates into more production capacity in $t=1$.

\begin{equation*}
	\max_{q^0,q^1}\Pi = (\alpha-\beta q^0)q^0 - cq^0 +  (\alpha-\beta q^1)q^1 - cq^1 -FI^0
\end{equation*}

subject to

\begin{eqnarray*}
	q^0 - K^0 &\leq& 0\\
	q^1 - K^1 &\leq& 0\\
        K^1 - K^0 - I^0 &=& 0\\
	q^0,q^1,I^0 &\geq& 0 
\end{eqnarray*}
 
We get the following Lagrangian.

\begin{eqnarray*}
	\mathcal{L}(q^0,q^1,\lambda^0,\lambda^1,\phi^1)&=& (\alpha-\beta q^0)q^0 - cq^0 +  (\alpha-\beta q^1)q^1 - cq^1 -FI^0 \\
        && - \lambda^0(q^0-K^0) - \lambda^1(q^1-K^1) - \phi^1(K^1-K^0-I^0)
\end{eqnarray*}

The KKT Conditions are as follows.

\begin{eqnarray*}
	0 \leq -\alpha + 2\beta q^0 + c + \lambda^0 &\bot& q^0 \geq 0\\
        0 \leq -\alpha + 2\beta q^1 + c + \lambda^1 &\bot& q^1 \geq 0\\
	0 \leq -q^0 + K^0 &\bot& \lambda^0 \geq 0 \\
        0 \leq -q^1 + K^1 &\bot& \lambda^1 \geq 0 \\
        0 = K^1 - K^0 - I^0 &\bot& \phi^1 \quad \mbox{free} \\
        0 \leq -\lambda^1 + \phi^1 &\bot& K^1 \geq 0 \\
        0 \leq F - \phi^1 &\bot& I^0 \geq 0 
\end{eqnarray*}


\subsection*{ex$\_$monopoly\_dyn.gms}

\lstinputlisting{ex_monopoly_dyn.gms}

\subsection*{ex$\_$monopoly\_.lst}

\lstinputlisting{ex_monopoly_dyn.lst}


\section{The simple monopoly goes dynamic (with better notation)}


We consider again the monopolist who produces with one technology. Now, we extend the time horizon to two stages, and allow for an investment in $t=0$, which translates into more production capacity in $t=1$.

\begin{equation*}
	\max_{q^t}\Pi = \sum_t\left[(\alpha-\beta q^t)q^t - cq^t  -FI^t\right]
\end{equation*}

subject to

\begin{eqnarray*}
	q^t - K^t &\leq& 0\quad \forall \,t\\
        K^{t+1} - K^t - I^t &=& 0 \quad \forall \, t>0\\
	q^t,I^t,K^t &\geq& 0 
\end{eqnarray*}
 
We get the following Lagrangian.

\begin{eqnarray*}
	\mathcal{L}(q^t,\lambda^t,\phi^t)&=& \sum_t\left[(\alpha-\beta q^t)q^t - cq^t  -FI^t\right] \\
        && \sum_{t\in T}- \lambda^t(q^t-K^t) - \sum_{t\in (T\backslash 0)}\phi^t(K^{t}-K^{t-1}-I^{t-1})
\end{eqnarray*}

The KKT Conditions are as follows.
 
\begin{eqnarray*}
	0 \leq -\alpha + 2\beta q^t + c + \lambda^t &\bot& q^t \geq 0 \quad\forall\,t\\
	0 \leq -q^t + K^t &\bot& \lambda^t \geq 0 \quad\forall\,t\\
        0 = K^{t} - K^{t-1} - I^{t-1} &\bot& \phi^t \quad \mbox{free}, \quad\forall\,t>0 \\
        0 \leq -\lambda^t + \phi^t &\bot& K^t \geq 0  \quad\forall\,t>0 \\
        0 \leq F - \phi^t &\bot& I^{t-1} \geq 0  \quad\forall\,t>0
\end{eqnarray*}


\subsection*{ex$\_$monopoly\_dyn.gms}

\lstinputlisting{ex_monopoly_dyn.gms}

\subsection*{ex$\_$monopoly\_.lst}

\lstinputlisting{ex_monopoly_dyn.lst}


\section{The dynamic monopoly with three stages}

We consider again the monopolist who produces with one technology. Now, we extend the time horizon to three stages, and allow for an investment in $t=0,1$, which translates into more production capacity in $t=1,2$.

\begin{equation*}
	\max_{q^0,q^1}\Pi = (\alpha-\beta q^0)q^0 - cq^0 +  (\alpha-\beta q^1)q^1 - cq^1 + (\alpha-\beta q^2)q^2 - cq^2 -FI^1
\end{equation*}

subject to

\begin{eqnarray*}
	q^0 - K^0 &\leq& 0\\
	q^1 - K^1 &\leq& 0\\
	q^2 - K^2 &\leq& 0\\
        K^1 - K^0 - I^0 &=& 0\\
        K^2 - K^1 - I^1 &=& 0\\
	q^0,q^1,q^1, I^0, I^1, K^0, K^1, K^2 &\geq& 0 
\end{eqnarray*}
 
We get the following Lagrangian.

\begin{eqnarray*}
	\mathcal{L}(q^0,q^1,q2,\lambda^0,\lambda^1,\lambda^2,\phi^1,\phi^2)&=& (\alpha-\beta q^0)q^0 - cq^0 +  (\alpha-\beta q^1)q^1 - cq^1 +  (\alpha-\beta q^2)q^2 - cq^2-FI^1 \\
        && - \lambda^0(q^0-K^0) - \lambda^1(q^1-K^1) - \lambda^1(q^2-K^2) \\
&& - \phi^1(K^1-K^0-I^0) - \phi^2(K^2-K^1-I^1)
\end{eqnarray*}

The KKT Conditions are as follows.

\begin{eqnarray*}
	0 \leq -\alpha + 2\beta q^0 + c + \lambda^0 &\bot& q^0 \geq 0\\
        0 \leq -\alpha + 2\beta q^1 + c + \lambda^1 &\bot& q^1 \geq 0\\
        0 \leq -\alpha + 2\beta q^2 + c + \lambda^2 &\bot& q^2 \geq 0\\
	0 \leq -q^0 + K^0 &\bot& \lambda^0 \geq 0 \\
        0 \leq -q^1 + K^1 &\bot& \lambda^1 \geq 0 \\
        0 \leq -q^2 + K^2 &\bot& \lambda^2 \geq 0 \\
        0 = K^1 - K^0 - I^0 &\bot& \phi^1 \quad \mbox{free} \\
        0 = K^2 - K^1 - I^1 &\bot& \phi^2 \quad \mbox{free} \\
        0 \leq -\lambda^1 + \phi^1 &\bot& K^1 \geq 0 \\
        0 \leq -\lambda^2 + \phi^2 &\bot& K^2 \geq 0 \\
        0 \leq F - \phi^1 &\bot& I^0 \geq 0 \\
        0 \leq F - \phi^2 &\bot& I^1 \geq 0 
\end{eqnarray*}


\subsection*{ex$\_$monopoly\_dyn\_stages.gms}

\lstinputlisting{ex_monopoly_dyn_3stages.gms}

%\subsection*{ex$\_$monopoly\_.lst}

%\lstinputlisting{ex_monopoly_dyn.lst}


\section{The simple monopoly with several technologies}

We continues with a static monopoly with several technologies. The monopolist has the following objective function:

\begin{equation*}
	\max_{q^j}\Pi = (\alpha-\beta \sum_{j\in M}q_j)\sum_{j\in M}q_j - \sum_{j\in M}c_jq_j 
\end{equation*}

subject to

\begin{eqnarray*}
	q_j - K_j &\leq& 0 \quad \forall\,j\\
	q_j, K_j &\geq& 0 \quad \forall\,j
\end{eqnarray*}
 
We get the following Lagrangian.

\begin{equation*}
	\mathcal{L}(q_j,\lambda_j)= (\alpha-\beta \sum_{j\in M}q_j)\sum_{j\in M}q_j - \sum_{j\in M}c_jq_j) - \sum_{j\in M} \lambda_j(q_j-K_j)
\end{equation*}

The KKT Conditions are as follows.

\begin{eqnarray*}
	0 \leq -\alpha + 2\beta \sum_{j\in M}q_j + c_j + \lambda_j &\bot& q_j \geq 0\quad \forall\,j\\
	0 \leq -q_j + K_j &\bot& \lambda_j \geq 0 \quad \forall\,j
\end{eqnarray*}


\subsection*{ex$\_$monopoly\_tech.gms}

\lstinputlisting{ex_monopoly_tech.gms}

\subsection*{ex$\_$monopoly\_tech.lst}

\lstinputlisting{ex_monopoly_tech.lst}

\section{The dynamic monopoly with several technologies}


We consider again the monopolist who produces with several technologies. Now, we extend the time horizon to two stages, and allow for an investment in $t=0$, which translates into more production capacity in $t=1$.

\begin{equation*}
	\max_{q_j^0,q_j^1}\Pi = (\alpha-\beta \sum_{j\in M}q_j^0)\sum_{j\in M}q_j^0 - \sum_{j\in M}c_jq_j^0 +  (\alpha-\beta \sum_{j\in M}q_j^1)\sum_{j\in M}q_j^1 - \sum_{j\in M}c_jq_j^1 - \sum_{j\in M}F_jI_j^0
\end{equation*}

subject to

\begin{eqnarray*}
	q_j^0 - K_j^0 &\leq& 0 \quad \forall\,j\\
	q_j^1 - K_j^1 &\leq& 0 \quad \forall\,j\\
        K_j^1 - K_j^0 - I_j^0 &=& 0 \quad \forall\,j\\
	q_j^0,q_j^1,I_j^0, K_j^0, K_j^1 &\geq& 0 \quad \forall\,j 
\end{eqnarray*}
 
We get the following Lagrangian.

\begin{eqnarray*}
	\mathcal{L}(q_j^0,q_j^1,\lambda_j^0,\lambda_j^1,\phi_j^1)&=& (\alpha-\beta \sum_{j\in M}q_j^0)\sum_{j\in M}q_j^0 - \sum_{j\in M}c_jq_j^0 \\
        && +  (\alpha-\beta \sum_{j\in M}q_j^1)\sum_{j\in M}q_j^1 - \sum_{j\in M}c_jq_j^1  - \sum_{j\in M}F_jI_j^0\\
        && - \sum_{j\in M}\lambda_j^0(q_j^0-K_j^0) - \sum_{j\in M}\lambda_j^1(q_j^1-K^1) - \sum_{j\in M}\phi_j^1(K_j^1-K_j^0-I_j^0)
\end{eqnarray*}

The KKT Conditions are as follows.

\begin{eqnarray*}
	0 \leq -\alpha + 2\beta \sum_{j\in M}q_j^0 + c_j + \lambda_j^0 &\bot& q_j^0 \geq 0\quad \forall\, j\\
	0 \leq -\alpha + 2\beta \sum_{j\in M}q_j^1 + c_j + \lambda_j^1 &\bot& q_j^1 \geq 0\quad \forall\, j\\
	0 \leq -q_j^0 + K_j^0 &\bot& \lambda_j^0 \geq 0 \quad \forall\, j \\
	0 \leq -q_j^1 + K_j^1 &\bot& \lambda_j^1 \geq 0 \quad \forall\, j \\
        0 = K_j^1 - K_j^0 - I_j^0 &\bot& \phi_j^1 \quad \mbox{free}  \quad \forall\, j\\
        0 \leq -\lambda_j^1 + \phi_j^1 &\bot& K_j^1 \geq 0  \quad \forall\, j\\
        0 \leq F_j - \phi_j^1 &\bot& I_j^0 \geq 0  \quad \forall\, j
\end{eqnarray*}


\subsection*{ex$\_$monopoly\_dyn\_tech.gms}

\lstinputlisting{ex_monopoly_dyn_tech.gms}

\subsection*{ex$\_$monopoly\_dyn\_tech.lst}

\lstinputlisting{ex_monopoly_dyn_tech.lst}


\section{The simple oligopoly}

Let us consider now a static oligopoly with one technology and $i$ different players. Each oligopolist has the following objective function:

\begin{equation*}
	\max_{q_i}\Pi_i = (\alpha-\beta \sum_{i\in N}q_i)q_i - cq_i 
\end{equation*}

subject to

\begin{eqnarray*}
	q_i - K_i &\leq& 0  \quad\forall\, i\\
	q_i,K_i &\geq& 0  \quad\forall\, i
\end{eqnarray*}
 
We get the following Lagrangian.

\begin{equation*}
	\mathcal{L}(q_i,\lambda_i)= (\alpha-\beta\sum_{i\in N} q_i)q_i - cq_i -\lambda_i(q_i-K_i)
\end{equation*}

The KKT Conditions are as follows.

\begin{eqnarray*}
	0 \leq -\alpha + \beta\sum_{i\in N} q_i + \beta q_i + c + \lambda_i &\bot& q_i \geq 0 \quad\forall\, i\\
	0 \leq -q_i + K_i &\bot& \lambda_i \geq 0 \quad\forall\, i
\end{eqnarray*}


\subsection*{ex$\_$oligopoly.gms}

\lstinputlisting{ex_oligopoly.gms}

\subsection*{ex$\_$oligopoly.lst}

\lstinputlisting{ex_oligopoly.lst}

\section{The dynamic oligopoly}


We consider again the oligopoly with $i$ players who produce with one technology. Now, we extend the time horizon to two stages, and allow for an investment in $t=0$, which translates into more production capacity in $t=1$.

\begin{equation*}
	\max_{q_i^0,q_i^1}\Pi_i = (\alpha-\beta \sum_{i\in N}q_i^0)q_i^0 - cq^0 +  (\alpha-\beta \sum_{i\in N}q_i^1)q_i^1 - cq_i^1 -FI_i^0
\end{equation*}

subject to

\begin{eqnarray*}
	q_i^0 - K_i^0 &\leq& 0 \quad\forall\, i\\
	q_i^1 - K_i^1 &\leq& 0 \quad\forall\, i\\
        K_i^1 - K_i^0 - I_i^0 &=& 0 \quad\forall\, i\\
	q_i^0,q_i^1,I_i^0, K_i^0, K_i^1 &\geq& 0 \quad\forall\, i
\end{eqnarray*}
 
We get the following Lagrangian.

\begin{eqnarray*}
	\mathcal{L}(q_i^0,q_i^1,\lambda_i^0,\lambda_i^1,\phi_i^1)&=&  (\alpha-\beta \sum_{i\in N}q_i^0)q_i^0 - cq^0 +  (\alpha-\beta \sum_{i\in N}q_i^1)q_i^1 - cq_i^1 -FI_i^0\\
        && - \lambda_i^0(q_i^0-K_i^0) - \lambda_i^1(q_i^1-K_i^1) - \phi_i^1(K_i^1-K_i^0-I_i^0)
\end{eqnarray*}

The KKT Conditions are as follows.

\begin{eqnarray*}
	0 \leq -\alpha + \beta \sum_{i\in N}q_i^0 + \beta q_i^0+ c + \lambda_i^0 &\bot& q_i^0 \geq 0\quad\forall\, i\\
	0 \leq -\alpha + \beta \sum_{i\in N}q_i^1 + \beta q_i^1+ c + \lambda_i^1 &\bot& q_i^1 \geq 0\quad\forall\, i\\
	0 \leq -q_i^0 + K_i^0 &\bot& \lambda_i^0 \geq 0 \quad\forall\, i \\
        0 \leq -q_i^1 + K_i^1 &\bot& \lambda_i^1 \geq 0 \quad\forall\, i\\
        0 = K_i^1 - K_i^0 - I_i^0 &\bot& \phi_i^1 \quad \mbox{free} \quad\forall\, i \\
        0 \leq -\lambda_i^1 + \phi_i^1 &\bot& K_i^1 \geq 0 \quad\forall\, i\\
        0 \leq F - \phi_i^1 &\bot& I_i^0 \geq 0 \quad\forall\, i
\end{eqnarray*}



\subsection*{ex$\_$oligopoly\_dyn.gms}

\lstinputlisting{ex_oligopoly_dyn.gms}

\subsection*{ex$\_$oligopoly\_dyn.lst}

\lstinputlisting{ex_oligopoly_dyn.lst}


\section{The dynamic oligopoly with several technologies}


We consider the oligopoly with $i$ players who produce with several technologies.

\begin{eqnarray*}
	\max_{q_{i,j}^0,q_{i,j}^1}\Pi_i &=& (\alpha-\beta \sum_{i\in N}\sum_{j\in M}q_{i,j}^0)\sum_{j\in M}q_{i,j}^0 - \sum_{j\in M}c_jq_{i,j}^0 \\
&& +  (\alpha-\beta \sum_{i\in N}\sum_{j\in M}q_{i,j}^1)\sum_{j\in M}q_i^1 - \sum_{j\in M}c_jq_{i,j}^1 - \sum_{j\in M}F_jI_{i,j}^0
\end{eqnarray*}

subject to

\begin{eqnarray*}
	q_{i,j}^0 - K_{i,j}^0 &\leq& 0 \quad\forall\, i,j\\
	q_{i,j}^1 - K_{i,j}^1 &\leq& 0 \quad\forall\, i,j\\
        K_{i,j}^1 - K_{i,j}^0 - I_{i,j}^0 &=& 0 \quad\forall\, i,j\\
	q_{i,j}^0,q_{i,j}^1,I_{i,j}^0, K_{i,j}^0, K_{i,j}^1 &\geq& 0 \quad\forall\, i,j
\end{eqnarray*}
 
We get the following Lagrangian.

\begin{eqnarray*}
	\mathcal{L}(q_i^0,q_i^1,\lambda_i^0,\lambda_i^1,\phi_i^1)&=&  (\alpha-\beta \sum_{i\in N}\sum_{j\in M}q_{i,j}^0)\sum_{j\in M}q_{i,j}^0 - \sum_{j\in M}c_jq_{i,j}^0 \\
&& +  (\alpha-\beta \sum_{i\in N}\sum_{j\in M}q_{i,j}^1)\sum_{j\in M}q_i^1 - \sum_{j\in M}c_jq_{i,j}^1 - \sum_{j\in M}F_jI_{i,j}^0\\
        && - \lambda_{i,j}^0(q_{i,j}^0-K_{i,j}^0) - \lambda_{i,j}^1(q_{i,j}^1-K_{i,j}^1) - \phi_{i,j}^1(K_{i,j}^1-K_{i,j}^0-I_{i,j}^0)
\end{eqnarray*}

The KKT Conditions are as follows.

\begin{eqnarray*}
	0 \leq -\alpha + \beta \sum_{i\in N}\sum_{j\in M}q_{i,j}^0 + \beta \sum_{j\in M}q_{i,j}^0+ c + \lambda_{i,j}^0 &\bot& q_{i,j}^0 \geq 0\quad\forall\, i,j\\
	0 \leq -\alpha + \beta \sum_{i\in N}\sum_{j\in M}q_{i,j}^1 + \beta\sum_{j\in M} q_{i,j}^1+ c + \lambda_{i,j}^1 &\bot& q_{i,j}^1 \geq 0\quad\forall\, i,j\\
	0 \leq -q_{i,j}^0 + K_{i,j}^0 &\bot& \lambda_{i,j}^0 \geq 0 \quad\forall\, i,j \\
        0 \leq -q_{i,j}^1 + K_{i,j}^1 &\bot& \lambda_{i,j}^1 \geq 0 \quad\forall\, i,j\\
        0 = K_{i,j}^1 - K_{i,j}^0 - I_{i,j}^0 &\bot& \phi_{i,j}^1 \quad \mbox{free} \quad\forall\, i,j \\
        0 \leq -\lambda_{i,j}^1 + \phi_{i,j}^1 &\bot& K_{i,j}^1 \geq 0 \quad\forall\, i,j\\
        0 \leq F - \phi_{i,j}^1 &\bot& I_{i,j}^0 \geq 0 \quad\forall\, i,j
\end{eqnarray*}

\subsection*{ex$\_$oligopoly\_dyn\_tech.gms}
\lstinputlisting{ex_oligopoly_dyn_tech.gms}

\subsection*{ex$\_$oligopoly\_dyn\_tech.lst}
\lstinputlisting{ex_oligopoly_dyn_tech.lst}

\section{The dynamic monopoly goes stochastic}


We consider again the monopolist who produces with one technology. The time horizon consists of two stages. In $t=1$ exist $s$ possible scenarios which occur with probability $p_s$. As there is only one investment decision made in $t=0$, a non-anticipativity constraint is not required. 

\begin{equation*}
	\max_{q^0,q^{s,1}}\Pi = (\alpha^0-\beta q^0)q^0 - cq^0 -FI^0 +  \sum_{s\in S}p_s\left[(\alpha^{s,1}-\beta q^{s,1})q^{s,1} - cq^{s,1}\right] 
\end{equation*}

subject to

\begin{eqnarray*}
	q^0 - K^0 &\leq& 0\\
	q^{s,1} - K^{1} &\leq& 0\quad\forall\, s\\
        K^{1} - K^0 - I^0 &=& 0\\
	q^0,q^{s,1},I^0,K^0,K^{1} &\geq& 0\quad\forall\, s 
\end{eqnarray*}
 
We get the following Lagrangian.

\begin{eqnarray*}
	\mathcal{L}(q^0,q^{s,1},\lambda^0,\lambda^{s,1},\phi^{s,1})&=& (\alpha^0-\beta q^0)q^0 - cq^0 - FI^0 + \sum_{s\in S}p_s\left[(\alpha^{s,1}-\beta q^{s,1})q^{s,1} - cq^{s,1}\right]  \\
        && - \lambda^0(q^0-K^0) - \sum_{s\in S}\lambda^{s,1}(q^{s,1}-K^{1}) - \phi^{1}(K^{1}-K^0-I^0)
\end{eqnarray*}

The KKT Conditions are as follows.

\begin{eqnarray*}
	0 \leq -\alpha^0 + 2\beta q^0 + c + \lambda^0 &\bot& q^0 \geq 0\\
        0 \leq -p_s\left(\alpha^{s,1} - 2\beta q^{s,1} - c\right) + \lambda^{s,1} &\bot& q^{s,1} \geq 0\quad\forall\,s\\
	0 \leq -q^0 + K^0 &\bot& \lambda^0 \geq 0 \\
        0 \leq -q^{s,1} + K^{1} &\bot& \lambda^{s,1} \geq 0 \quad\forall\,s\\
        0 = K^1 - K^0 - I^0 &\bot& \phi^1 \quad \mbox{free} \\
        0 \leq -\sum_{s\in S}\lambda^{s,1} + \phi^{1} &\bot& K^1 \geq 0 \\
        0 \leq F - \phi^{1} &\bot& I^0 \geq 0 
\end{eqnarray*}

\subsection*{ex$\_$monopoly\_dyn\_stoch.gms}
\lstinputlisting{ex_monopoly_dyn_stoch.gms}

\subsection*{ex$\_$monopoly\_dyn\_stoch.lst}
\lstinputlisting{ex_monopoly_dyn_stoch.lst}

\section{The dynamic stochastic monopoly with three stages}


We consider again the monopolist who produces with one technology. The time horizon consists of three stages. There exist $s$ possible scenarios which occur with probability $p_s$. As there two investment decisions are made, non-anticipativity constraints are required. For $t=0,\dots,2$ we get a scenario tree with $2^2=4$ scenarios, with a probability of each scenario $p_s=1/4=0.25$.

\begin{eqnarray*}
	\max_{q^0,q^{s,1},q^{s,2},I^0,I^{s,1}}\Pi &=& (\alpha^0-\beta q^0)q^0 - cq^0 -FI^0  \\
        && + p_s\left[(\alpha^{1,1}-\beta q^{1,1})q^{1,1} - cq^{1,1} - FI^{1,1} + (\alpha^{1,2}-\beta q^{1,2})q^{1,2} - cq^{1,2}\right] \\
        && + p_s\left[(\alpha^{2,1}-\beta q^{2,1})q^{2,1} - cq^{2,1} - FI^{2,1} + (\alpha^{2,2}-\beta q^{2,2})q^{2,2} - cq^{2,2}\right] \\
        && + p_s\left[(\alpha^{3,1}-\beta q^{3,1})q^{3,1} - cq^{3,1} - FI^{3,1} + (\alpha^{3,2}-\beta q^{3,2})q^{3,2} - cq^{3,2}\right] \\
        && + p_s\left[(\alpha^{4,1}-\beta q^{4,1})q^{4,1} - cq^{4,1} - FI^{4,1} + (\alpha^{4,2}-\beta q^{4,2})q^{4,2} - cq^{4,2}\right] 
\end{eqnarray*}

subject to

\begin{eqnarray*}
	q^0 - K^0 &\leq& 0\\
	q^{1,1} - K^{1} &\leq& 0\\
        q^{2,1} - K^{1} &\leq& 0\\
        q^{3,1} - K^{1} &\leq& 0\\
        q^{4,1} - K^{1} &\leq& 0\\
	q^{1,2} - K^{1,2} &\leq& 0\\
	q^{2,2} - K^{2,2} &\leq& 0\\
	q^{3,2} - K^{3,2} &\leq& 0\\
	q^{4,2} - K^{4,2} &\leq& 0\\
        K^{1} - K^0 - I^0 &=& 0\\
        K^{1,2} - K^1 - I^{1,1} &=& 0\\
        K^{2,2} - K^1 - I^{2,1} &=& 0\\
        K^{3,2} - K^1 - I^{3,1} &=& 0\\
        K^{4,2} - K^1 - I^{4,1} &=& 0\\
        I^{1,1} &=& I^{1,2} \\
        I^{1,3} &=& I^{1,4} \\
	q^0,q^{s,1},q^{s,2},I^0,I^{s,1},K^0,K^{1},K^{s,2} &\geq& 0\quad\forall\, s 
\end{eqnarray*}
 
We get the following Lagrangian.

\begin{eqnarray*}
	\mathcal{L}(q^0,q^{s,1},q^{s,2},I^0,I^{s,1},I^{s,2},\lambda^0,\lambda^{s,1},\lambda^{s,2},\phi^{s,1},\phi^{s,2})= (\alpha^0-\beta q^0)q^0 - cq^0 - FI^0 \\
        + p_s\left[(\alpha^{1,1}-\beta q^{1,1})q^{1,1} - cq^{1,1} - FI^{1,1} + (\alpha^{1,2}-\beta q^{1,2})q^{1,2} - cq^{1,2}\right] \\
        + p_s\left[(\alpha^{2,1}-\beta q^{2,1})q^{2,1} - cq^{2,1} - FI^{2,1} + (\alpha^{2,2}-\beta q^{2,2})q^{2,2} - cq^{2,2}\right] \\
        + p_s\left[(\alpha^{3,1}-\beta q^{3,1})q^{3,1} - cq^{3,1} - FI^{3,1} + (\alpha^{3,2}-\beta q^{3,2})q^{3,2} - cq^{3,2}\right] \\
        + p_s\left[(\alpha^{4,1}-\beta q^{4,1})q^{4,1} - cq^{4,1} - FI^{4,1} + (\alpha^{4,2}-\beta q^{4,2})q^{4,2} - cq^{4,2}\right] \\
         - \lambda^0(q^0-K^0) - \sum_{s\in S}\lambda^{s,1}(q^{s,1}-K^{1}) - \phi^{1}(K^{1}-K^0-I^0) \\
- \sum_{s\in S}\lambda^{s,2}(q^{s,2}-K^{s,2}) - \sum_{s\in S}\phi^{s,2}(K^{s,2}-K^1-I^{s,1})\\
- \psi^{1}(I^{1,1} - I^{1,2}) - \psi^{2}(I^{1,3} - I^{1,4})\\
\end{eqnarray*}

The KKT Conditions are as follows.

\begin{eqnarray*}
	0 \leq -\alpha^0 + 2\beta q^0 + c + \lambda^0 &\bot& q^0 \geq 0\\
        0 \leq -p_s\left(\alpha^{s,1} - 2\beta q^{s,1} - c\right) + \lambda^{s,1} &\bot& q^{s,1} \geq 0\quad\forall\,s\\
       0 \leq -p_s\left(\alpha^{s,2} - 2\beta q^{s,2} - c\right) + \lambda^{s,2} &\bot& q^{s,2} \geq 0\quad\forall\,s\\
	0 \leq -q^0 + K^0 &\bot& \lambda^0 \geq 0 \\
        0 \leq -q^{s,1} + K^{1} &\bot& \lambda^{s,1} \geq 0 \quad\forall\,s\\
        0 \leq -q^{s,2} + K^{s,2} &\bot& \lambda^{s,2} \geq 0 \quad\forall\,s\\
        0 = K^1 - K^0 - I^0 &\bot& \phi^1 \quad \mbox{free} \\
        0 = K^{s,2} - K^1 - I^{s,1} &\bot& \phi^{s,2} \quad \mbox{free}\quad\forall\,s \\
        0 \leq -\sum_{s\in S}\lambda^{s,1} + \phi^{1}-\sum_{s\in S}\phi^{s,2} &\bot& K^1 \geq 0 \\
        0 \leq -\sum_{s\in S}\lambda^{s,2} + \sum_{s\in S}\phi^{s,2} &\bot& K^{s,2} \geq 0\quad\forall\,s \\
        0 \leq F - \phi^{1} &\bot& I^0 \geq 0\\
        0 \leq p_sF - \phi^{1,2} + \psi^1 &\bot& I^{1,1} \geq 0 \\
        0 \leq p_sF - \phi^{2,2} - \psi^1 &\bot& I^{2,1} \geq 0 \\
        0 \leq p_sF - \phi^{3,2} + \psi^2 &\bot& I^{3,1} \geq 0 \\
        0 \leq p_sF - \phi^{4,2} - \psi^2&\bot& I^{4,1} \geq 0 \\
        0 = I^{1,1}-I^{2,1}&\bot& \psi^1\quad \mbox{free} \\
        0 = I^{3,1}-I^{4,1}&\bot& \psi^2\quad \mbox{free} \\
\end{eqnarray*}
KKTs with non-anticipativity constraints don't work yet. An alternative would be the compact formulation used in Zhuang and Gabriel (2008).

Compact formulation

\begin{eqnarray*}
	\max_{q^0,q^{s,1},q^{s,2},I^0,I^{s,1}}\Pi &=& (\alpha^{n0}-\beta q^{n0})q^{n0} - cq^{n0} -FI^{n0}  \\
        && + 0.5\delta_1\left[(\alpha^{n1}-\beta q^{n1})q^{n1} - cq^{n1} - FI^{n1}\right] \\
        && + 0.5\delta_1\left[(\alpha^{n2}-\beta q^{n2})q^{n2} - cq^{n2} - FI^{n2}\right] \\
        && + 0.25\delta_2\left[(\alpha^{n3}-\beta q^{n3})q^{n3} - cq^{n3} + FK^{n3}\nu\right] \\
        && + 0.25\delta_2\left[(\alpha^{n4}-\beta q^{n4})q^{n4} - cq^{n4} + FK^{n4}\nu\right] \\
        && + 0.25\delta_2\left[(\alpha^{n5}-\beta q^{n5})q^{n5} - cq^{n5} + FK^{n5}\nu\right] \\
        && + 0.25\delta_2\left[(\alpha^{n6}-\beta q^{n6})q^{n6} - cq^{n6} + FK^{n6}\nu\right] \\
\end{eqnarray*}
\begin{eqnarray*}
	q^{n0} - K^0 &\leq& 0\\
	q^{n1} - K^{n1} &\leq& 0\\
        q^{n2} - K^{n2} &\leq& 0\\
        q^{n3} - K^{n3} &\leq& 0\\
        q^{n4} - K^{n4} &\leq& 0\\
	q^{n5} - K^{n5} &\leq& 0\\
	q^{n6} - K^{n6} &\leq& 0\\
        K^{n1} - (1-r)K^0 - I^{n0} &=& 0\\
        K^{n2} - (1-r)K^0 - I^{n0} &=& 0\\
        K^{n3} - (1-r)K^{n1} - I^{n1} &=& 0\\
        K^{n4} - (1-r)K^{n2} - I^{n1} &=& 0\\
        K^{n5} - (1-r)K^{n2} - I^{n2} &=& 0\\
        K^{n6} - (1-r)K^{n2} - I^{n2} &=& 0\\
\end{eqnarray*}
\begin{eqnarray*}
	0 \leq -\alpha^{n0} + 2\beta q^{n0} + c + \lambda^{n0} &\bot& q^{n0} \geq 0\\
        0 \leq -0.5\left(\alpha^{n1} - 2\beta q^{n1} - c\right) + \lambda^{n1} &\bot& q^{n1} \geq 0\\
        0 \leq -0.5\left(\alpha^{n2} - 2\beta q^{n2} - c\right) + \lambda^{n2} &\bot& q^{n2} \geq 0\\
        0 = K^{n1}-K^0-I^{n0}  &\bot& \phi^{n1} \quad\mbox{free}\\
        0 = K^{n2}-K^0-I^{n0}  &\bot& \phi^{n2} \quad\mbox{free}\\
	0 \leq -q^{n0} + K^{0} &\bot& \lambda^{n0} \geq 0\\
	0 \leq -q^{n1} + K^{n1} &\bot& \lambda^{n1} \geq 0\\
	0 \leq -q^{n2} + K^{n2} &\bot& \lambda^{n2} \geq 0\\
	0 \leq F-\phi^{n1}-\phi^{n2} &\bot& I^{n0} \geq 0\\
	0 \leq -\lambda^{n1}\phi^{n1} &\bot& K^{n1} \geq 0\\
        0 \leq -\lambda^{n2}\phi^{n2}  &\bot& K^{n2} \geq 0\\
\end{eqnarray*}


\section{The simple monopoly with a price-cap}

We consider a static monopoly with one technology. A price cap $\bar{p}$ is imposed. The monopolist has the following objective function:

\begin{equation*}
	\max_q\Pi = (\alpha-\beta q)q - cq 
\end{equation*}

subject to

\begin{eqnarray*}
	q - K &\leq& 0\\
        \alpha-\beta q - \bar{p} &\leq& 0 \\ 
	q &\geq& 0 
\end{eqnarray*}
 
We get the following Lagrangian.

\begin{equation*}
	\mathcal{L}(q,\lambda)= (\alpha-\beta q)q - cq -\lambda(q-K) - \psi\left(\alpha-\beta q-\bar{p}\right)
\end{equation*}

The KKT Conditions are as follows.

\begin{eqnarray*}
	0 \leq -\alpha + 2\beta q + c + \lambda - \psi\beta &\bot& q \geq 0\\
	0 \leq -q + K &\bot& \lambda \geq 0\\
        0 \leq - \alpha + \beta q + \bar{p}  &\bot& \psi \geq 0
\end{eqnarray*}

We consider a static monopoly with one technology. A price cap $\bar{p}$ is imposed. The monopolist has the following objective function:

\begin{equation*}
	\max_q\Pi = \min\left[(\alpha-\beta q),\bar{p}\right]q - cq 
\end{equation*}

subject to

\begin{eqnarray*}
	q - K &\leq& 0\\
        \alpha-\beta q - \bar{p} &\leq& 0 \\ 
	q &\geq& 0 
\end{eqnarray*}
 
We get the following Lagrangian.

\begin{equation*}
	\mathcal{L}(q,\lambda)= (\alpha-\beta q)q - cq -\lambda(q-K) - \psi\left(\alpha-\beta q-\bar{p}\right)
\end{equation*}

The KKT Conditions are as follows.

\begin{eqnarray*}
	0 \leq -\alpha + 2\beta q + c + \lambda - \psi\beta &\bot& q \geq 0\\
	0 \leq -q + K &\bot& \lambda \geq 0\\
        0 \leq - \alpha + \beta q + \bar{p}  &\bot& \psi \geq 0
\end{eqnarray*}

\subsection*{ex$\_$monopoly\_pc.gms}
\lstinputlisting{ex_monopoly_pc.gms}

\subsection*{ex$\_$monopoly\_pc.lst}
\lstinputlisting{ex_monopoly_pc.lst}

Not working, objective function is discontinous.

\section{The dynamic stochastic monopoly with scrap values}


We consider again the monopolist who produces with one technology. The time horizon consists of two stages. In $t=1$ exist $s$ possible scenarios which occur with probability $p_s$. As there is only one investment decision made in $t=0$, a non-anticipativity constraint is not required. 

\begin{equation*}
	\max_{q^0,q^{s,1}}\Pi = (\alpha^0-\beta q^0)q^0 - cq^0 -FI^0 +  \sum_{s\in S}p_s\left[(\alpha^{s,1}-\beta q^{s,1})q^{s,1} - cq^{s,1} + FK^1\right] 
\end{equation*}

subject to

\begin{eqnarray*}
	q^0 - K^0 &\leq& 0\\
	q^{s,1} - K^{1} &\leq& 0\quad\forall\, s\\
        K^{1} - K^0 - I^0 &=& 0\\
	q^0,q^{s,1},I^0,K^0,K^{1} &\geq& 0\quad\forall\, s 
\end{eqnarray*}
 
We get the following Lagrangian.

\begin{eqnarray*}
	\mathcal{L}(q^0,q^{s,1},\lambda^0,\lambda^{s,1},\phi^{s,1})&=& (\alpha^0-\beta q^0)q^0 - cq^0 - FI^0 + \sum_{s\in S}p_s\left[(\alpha^{s,1}-\beta q^{s,1})q^{s,1} - cq^{s,1} + FK^1\right]  \\
        && - \lambda^0(q^0-K^0) - \sum_{s\in S}\lambda^{s,1}(q^{s,1}-K^{1}) - \phi^{1}(K^{1}-K^0-I^0)
\end{eqnarray*}

The KKT Conditions are as follows.

\begin{eqnarray*}
	0 \leq -\alpha^0 + 2\beta q^0 + c + \lambda^0 &\bot& q^0 \geq 0\\
        0 \leq -p_s\left(\alpha^{s,1} - 2\beta q^{s,1} - c\right) + \lambda^{s,1} &\bot& q^{s,1} \geq 0\quad\forall\,s\\
	0 \leq -q^0 + K^0 &\bot& \lambda^0 \geq 0 \\
        0 \leq -q^{s,1} + K^{1} &\bot& \lambda^{s,1} \geq 0 \quad\forall\,s\\
        0 = K^1 - K^0 - I^0 &\bot& \phi^1 \quad \mbox{free} \\
        0 \leq -F -\sum_{s\in S}\lambda^{s,1} + \phi^{1} &\bot& K^1 \geq 0 \\
        0 \leq F - \phi^{1} &\bot& I^0 \geq 0 
\end{eqnarray*}

\end{document}